@prefix : <http://www.owlsai.com/ontologies/controlsystem#> .
@prefix owl: <http://www.w3.org/2002/07/owl#> .
@prefix rdf: <http://www.w3.org/1999/02/22-rdf-syntax-ns#> .
@prefix xml: <http://www.w3.org/XML/1998/namespace> .
@prefix xsd: <http://www.w3.org/2001/XMLSchema#> .
@prefix rdfs: <http://www.w3.org/2000/01/rdf-schema#> .

<http://www.owlsai.com/ontologies/controlsystem> a owl:Ontology ;
	owl:imports <http://www.owlsai.com/ontologies/situation> ;
	<http://purl.org/dc/terms/abstract> """The Control System Module Ontology is designed to describe those things we model as Control Systems by extending the Systems and Situations Modules.

It includes definitions for Actuators, Sensors and Controllers, these Systems are not considered disjoint to permit a user to describe one system that has all of the associated capabilities without requiring them to decompose them into the respective Actuator, Sensor and Controller parts."""@en ;
	<http://purl.org/dc/terms/created> "2019-03-14" ;
	<http://purl.org/dc/terms/creator> <http://www.paulbrownmagic.com/foaf#me> ;
	<http://purl.org/dc/terms/license> <https://mit-license.org/> ;
	<http://purl.org/dc/terms/title> "Control Systems Ontology Module"@en ;
	<http://purl.org/vocab/vann/preferredNamespacePrefix> "csys"@en ;
	<http://purl.org/vocab/vann/preferredNamespaceUri> "http://www.owlsai.com/ontologies/controlsystem#"@en ;
	rdfs:comment "An ontology module for describing control systems."@en ;
	owl:versionInfo "1.0.0" .
# 
# 
# #################################################################
# #
# #    Object Properties
# #
# #################################################################
# 
# 
# http://www.owlsai.com/ontologies/controlsystem#believesHolds

:believesHolds a owl:ObjectProperty ;
	rdfs:domain :ProcessModel ;
	rdfs:range <http://www.owlsai.com/ontologies/situation#Fluent> ;
	rdfs:comment "ProcessModel believesHolds Fluent means the Process model believes but cannot be certain the Fluent holds in the current Situation."@en ;
	rdfs:label "believes holds"@en .
# 
# http://www.owlsai.com/ontologies/controlsystem#hasComponent

:hasComponent a owl:ObjectProperty ;
	owl:inverseOf :isComponentOf ;
	a owl:TransitiveProperty ;
	rdfs:domain :System ;
	rdfs:range <http://www.owlsai.com/ontologies/tinytop#Entity> ;
	rdfs:comment """Integral hasComponent Component.

\"Integral objects all exhibit some kind of patterned organization or structure. Their components are also patterned and usually bear specific structural and functional relationships to one another and to the wholes which they compose. These structural relations define the particular natures of integral wholes and their components -- components cannot be haphazardly arranged but must be arranged in a particular patterned organization within the wholes they comprise\"
(Source: Winston, Chaffin and Herrmann, 1987)

eg:
    Car hasComponent Wheel"""@en ;
	rdfs:label "has component"@en .
# 
# http://www.owlsai.com/ontologies/controlsystem#hasDirectComponent

:hasDirectComponent a owl:ObjectProperty ;
	rdfs:subPropertyOf :hasComponent ;
	owl:inverseOf :isDirectComponentOf ;
	rdfs:domain :System ;
	rdfs:range <http://www.owlsai.com/ontologies/tinytop#Entity> ;
	rdfs:comment "As per hasComponent, but not transitive. Expresses granularity."@en ;
	rdfs:label "has direct component"@en .
# 
# http://www.owlsai.com/ontologies/controlsystem#isComponentOf

:isComponentOf a owl:ObjectProperty , owl:TransitiveProperty ;
	rdfs:domain <http://www.owlsai.com/ontologies/tinytop#Entity> ;
	rdfs:range :System ;
	rdfs:comment """Component isComponentOf Integral.

\"Integral objects all exhibit some kind of patterned organization or structure. Their components are also patterned and usually bear specific structural and functional relationships to one another and to the wholes which they compose. These structural relations define the particular natures of integral wholes and their components -- components cannot be haphazardly arranged but must be arranged in a particular patterned organization within the wholes they comprise\"
(Source: Winston, Chaffin and Herrmann, 1987)

e.g.
    Wheel isComponentOf Car"""@en ;
	rdfs:label "is component of"@en .
# 
# http://www.owlsai.com/ontologies/controlsystem#isDirectComponentOf

:isDirectComponentOf a owl:ObjectProperty ;
	rdfs:subPropertyOf :isComponentOf ;
	rdfs:domain <http://www.owlsai.com/ontologies/tinytop#Entity> ;
	rdfs:range :System ;
	rdfs:comment "As per isComponentOf but not transitive. Expresses granularity."@en ;
	rdfs:label "is direct component of"@en .
# 
# http://www.owlsai.com/ontologies/controlsystem#isRealizedIn

:isRealizedIn a owl:ObjectProperty ;
	owl:inverseOf :realizes ;
	rdfs:domain <http://www.owlsai.com/ontologies/tinytop#Capability> ;
	rdfs:range <http://www.owlsai.com/ontologies/tinytop#Process> ;
	rdfs:comment "Capability isRealizedIn Process means there is some Entity that hasCapability Capability and that Entity is realized or occurs in that Process"@en ;
	rdfs:label "is realized in"@en ;
	rdfs:seeAlso "http://purl.obolibrary.org/obo/BFO_0000054" .
# 
# http://www.owlsai.com/ontologies/controlsystem#observes

:observes a owl:ObjectProperty ;
	rdfs:domain :Observation ;
	rdfs:range <http://www.owlsai.com/ontologies/situation#Fluent> ;
	rdfs:comment "Observation observes Fluent means that realizing that Observation measures if that Fluent holds in a Situation. No presumption of accuracy is made, only the attempt to measure."@en ;
	rdfs:label "observes"@en .
# 
# http://www.owlsai.com/ontologies/controlsystem#realizes

:realizes a owl:ObjectProperty ;
	rdfs:domain <http://www.owlsai.com/ontologies/tinytop#Process> ;
	rdfs:range <http://www.owlsai.com/ontologies/tinytop#Capability> ;
	rdfs:comment "Process realizes Capability means there is some Entity that hasCapability Capability and that Entity is realized or occurs in that Process"@en ;
	rdfs:label "realizes"@en ;
	rdfs:seeAlso "http://purl.obolibrary.org/obo/BFO_0000055" .
# 
# http://www.owlsai.com/ontologies/controlsystem#receivesFeedback

:receivesFeedback a owl:ObjectProperty ;
	rdfs:subPropertyOf <http://www.owlsai.com/ontologies/tinytop#informedBy> ;
	rdfs:domain :Controller ;
	rdfs:range :Feedback ;
	rdfs:comment "Controller receivesFeedback Feedback means the Controller reads the information contained within the feedback."@en ;
	rdfs:label "receives feedback"@en .
# 
# http://www.owlsai.com/ontologies/controlsystem#recordsResultOf

:recordsResultOf a owl:ObjectProperty ;
	owl:inverseOf :resultRecordedIn ;
	rdfs:domain :Feedback ;
	rdfs:range :Observation ;
	rdfs:comment "Feedback recordsResultOf Observation means the Feedback describes the Fluent as observed in the Situation when the Observation is realized by the Sensor."@en ;
	rdfs:label "records result of"@en .
# 
# http://www.owlsai.com/ontologies/controlsystem#requests

:requests a owl:ObjectProperty ;
	rdfs:domain :ControlAction ;
	rdfs:range :Actuation ;
	rdfs:comment "Controller requests Acutation means the Controller can realize in some Process a request for an Actuator to perform an Actuation and bring about some transition between Situations"@en ;
	rdfs:label "requests"@en .
# 
# http://www.owlsai.com/ontologies/controlsystem#resultRecordedIn

:resultRecordedIn a owl:ObjectProperty ;
	rdfs:domain :Observation ;
	rdfs:range :Feedback ;
	rdfs:comment "Observation resultRecordedIn Feedback means the Feedback describes the Fluent as observed in the Situation when the Observation is realized by the Sensor."@en ;
	rdfs:label "result recorded in"@en .
# 
# 
# 
# #################################################################
# #
# #    Classes
# #
# #################################################################
# 
# 
# http://www.owlsai.com/ontologies/controlsystem#Actuation

:Actuation a owl:Class ;
	owl:equivalentClass _:genid1 .

_:genid1 owl:intersectionOf _:genid4 .

_:genid4 a rdf:List ;
	rdf:first <http://www.owlsai.com/ontologies/tinytop#Capability> ;
	rdf:rest _:genid2 .

_:genid2 a rdf:List ;
	rdf:first _:genid3 .

_:genid3 a owl:Restriction ;
	owl:onProperty <http://www.owlsai.com/ontologies/situation#hasEffect> ;
	owl:someValuesFrom <http://www.owlsai.com/ontologies/situation#Fluent> .

_:genid2 rdf:rest rdf:nil .

_:genid1 a owl:Class .

:Actuation rdfs:comment "An Actuation is the capability to transition to a new Situation by changing which Fluents hold."@en ;
	rdfs:label "Actuation"@en .
# 
# http://www.owlsai.com/ontologies/controlsystem#Actuator

:Actuator a owl:Class ;
	owl:equivalentClass _:genid5 .

_:genid5 owl:intersectionOf _:genid8 .

_:genid8 a rdf:List ;
	rdf:first :System ;
	rdf:rest _:genid6 .

_:genid6 a rdf:List ;
	rdf:first _:genid7 .

_:genid7 a owl:Restriction ;
	owl:onProperty <http://www.owlsai.com/ontologies/tinytop#hasCapability> ;
	owl:someValuesFrom :Actuation .

_:genid6 rdf:rest rdf:nil .

_:genid5 a owl:Class .

:Actuator rdfs:comment "An Actuator is a System with the Capability for Actuation, which causes some Fluent to hold, i.e. it causes change by transitioning to new Situations"@en ;
	rdfs:label "Actuator"@en ;
	rdfs:seeAlso "http://www.w3.org/ns/sosa/Actuator" .
# 
# http://www.owlsai.com/ontologies/controlsystem#ControlAction

:ControlAction a owl:Class ;
	owl:equivalentClass _:genid9 .

_:genid9 owl:intersectionOf _:genid12 .

_:genid12 a rdf:List ;
	rdf:first <http://www.owlsai.com/ontologies/tinytop#Capability> ;
	rdf:rest _:genid10 .

_:genid10 a rdf:List ;
	rdf:first _:genid11 .

_:genid11 a owl:Restriction ;
	owl:onProperty :requests ;
	owl:someValuesFrom :Actuation .

_:genid10 rdf:rest rdf:nil .

_:genid9 a owl:Class .

:ControlAction rdfs:comment "A Control Action is the Capability to request that some Actuation be realized in a Process."@en ;
	rdfs:label "Control Action"@en .
# 
# http://www.owlsai.com/ontologies/controlsystem#Controller

:Controller a owl:Class ;
	owl:equivalentClass _:genid13 .

_:genid13 owl:intersectionOf _:genid22 .

_:genid22 a rdf:List ;
	rdf:first :System ;
	rdf:rest _:genid20 .

_:genid20 a rdf:List ;
	rdf:first _:genid21 .

_:genid21 a owl:Restriction ;
	owl:onProperty :receivesFeedback ;
	owl:someValuesFrom :Feedback .

_:genid20 rdf:rest _:genid18 .

_:genid18 a rdf:List ;
	rdf:first _:genid19 .

_:genid19 a owl:Restriction ;
	owl:onProperty <http://www.owlsai.com/ontologies/tinytop#hasCapability> ;
	owl:someValuesFrom :ControlAction .

_:genid18 rdf:rest _:genid16 .

_:genid16 a rdf:List ;
	rdf:first _:genid17 .

_:genid17 a owl:Restriction ;
	owl:onProperty <http://www.owlsai.com/ontologies/tinytop#informedBy> ;
	owl:someValuesFrom :Procedure .

_:genid16 rdf:rest _:genid14 .

_:genid14 a rdf:List ;
	rdf:first _:genid15 .

_:genid15 a owl:Restriction ;
	owl:onProperty <http://www.owlsai.com/ontologies/tinytop#informedBy> ;
	owl:someValuesFrom :ProcessModel .

_:genid14 rdf:rest rdf:nil .

_:genid13 a owl:Class .

:Controller rdfs:comment "Uses internal process model and sensed information to make decisions regarding its initiation of control actions."@en ;
	rdfs:label "Controller"@en .
# 
# http://www.owlsai.com/ontologies/controlsystem#Feedback

:Feedback a owl:Class ;
	rdfs:subClassOf <http://www.owlsai.com/ontologies/tinytop#InformationEntity> ;
	rdfs:comment "Feedback is an information content entity that is intended to inform some decision making process"@en ;
	rdfs:label "Feedback"@en .
# 
# http://www.owlsai.com/ontologies/controlsystem#Observation

:Observation a owl:Class ;
	owl:equivalentClass _:genid23 .

_:genid23 owl:intersectionOf _:genid26 .

_:genid26 a rdf:List ;
	rdf:first <http://www.owlsai.com/ontologies/tinytop#Capability> ;
	rdf:rest _:genid24 .

_:genid24 a rdf:List ;
	rdf:first _:genid25 .

_:genid25 a owl:Restriction ;
	owl:onProperty :observes ;
	owl:someValuesFrom <http://www.owlsai.com/ontologies/situation#Fluent> .

_:genid24 rdf:rest rdf:nil .

_:genid23 a owl:Class .

:Observation rdfs:comment "Observation is the Capability to measure if a Fluent holds in a Situation"@en ;
	rdfs:label "Observation"@en .
# 
# http://www.owlsai.com/ontologies/controlsystem#Procedure

:Procedure a owl:Class ;
	rdfs:subClassOf <http://www.owlsai.com/ontologies/tinytop#InformationEntity> ;
	rdfs:comment "A Procedure is an algorithm, heuristic, workflow, protocol or plan outlining some Process"@en ;
	rdfs:label "Procedure"@en .
# 
# http://www.owlsai.com/ontologies/controlsystem#ProcessModel

:ProcessModel a owl:Class ;
	rdfs:subClassOf <http://www.owlsai.com/ontologies/tinytop#InformationEntity> ;
	rdfs:comment "A ProcessModel is a model of a process held by some observer of the process. It may not be accurate."@en ;
	rdfs:label "Process Model"@en .
# 
# http://www.owlsai.com/ontologies/controlsystem#Sensor

:Sensor a owl:Class ;
	owl:equivalentClass _:genid27 .

_:genid27 owl:intersectionOf _:genid30 .

_:genid30 a rdf:List ;
	rdf:first :System ;
	rdf:rest _:genid28 .

_:genid28 a rdf:List ;
	rdf:first _:genid29 .

_:genid29 a owl:Restriction ;
	owl:onProperty <http://www.owlsai.com/ontologies/tinytop#hasCapability> ;
	owl:someValuesFrom :Observation .

_:genid28 rdf:rest rdf:nil .

_:genid27 a owl:Class .

:Sensor rdfs:comment "A Sensor is a System that can measure a Fluent, i.e. check if a Fluent holds in the current Situation."@en ;
	rdfs:label "Sensor"@en ;
	rdfs:seeAlso "http://www.w3.org/ns/sosa/Sensor" .
# 
# http://www.owlsai.com/ontologies/controlsystem#System

:System a owl:Class ;
	owl:equivalentClass _:genid31 .

_:genid31 owl:intersectionOf _:genid34 .

_:genid34 a rdf:List ;
	rdf:first <http://www.owlsai.com/ontologies/tinytop#Entity> ;
	rdf:rest _:genid32 .

_:genid32 a rdf:List ;
	rdf:first _:genid33 .

_:genid33 a owl:Restriction ;
	owl:onProperty :hasComponent ;
	owl:someValuesFrom <http://www.owlsai.com/ontologies/tinytop#Entity> .

_:genid32 rdf:rest rdf:nil .

_:genid31 a owl:Class .

:System rdfs:comment """A complex whole comprised of an organisation of parts.

Each part may be a system. It affects and is affected by its environment. An object that can be understood by decomposing it into its component parts."""@en ;
	rdfs:label "System"@en .
# 
# http://www.owlsai.com/ontologies/controlsystem#SystemQuality

:SystemQuality a owl:Class ;
	owl:equivalentClass _:genid35 .

_:genid35 owl:intersectionOf _:genid38 .

_:genid38 a rdf:List ;
	rdf:first <http://www.owlsai.com/ontologies/situation#QualityFluent> ;
	rdf:rest _:genid36 .

_:genid36 a rdf:List ;
	rdf:first _:genid37 .

_:genid37 a owl:Restriction ;
	owl:onProperty <http://www.owlsai.com/ontologies/situation#hasBearer> ;
	owl:someValuesFrom :System .

_:genid36 rdf:rest rdf:nil .

_:genid35 a owl:Class .

:SystemQuality owl:equivalentClass _:genid39 .

_:genid39 owl:intersectionOf _:genid44 .

_:genid44 a rdf:List ;
	rdf:first <http://www.owlsai.com/ontologies/situation#QualityFluent> ;
	rdf:rest _:genid42 .

_:genid42 a rdf:List ;
	rdf:first _:genid43 .

_:genid43 a owl:Restriction ;
	owl:onProperty <http://www.owlsai.com/ontologies/situation#hasBearer> ;
	owl:someValuesFrom :System .

_:genid42 rdf:rest _:genid40 .

_:genid40 a rdf:List ;
	rdf:first _:genid41 .

_:genid41 a owl:Restriction ;
	owl:onProperty <http://www.owlsai.com/ontologies/situation#hasQualityInSomeSituation> ;
	owl:someValuesFrom <http://www.owlsai.com/ontologies/tinytop#Quality> .

_:genid40 rdf:rest rdf:nil .

_:genid39 a owl:Class .

:SystemQuality rdfs:label "System Quality"@en .
# 
# Generated by the OWL API (version 4.5.9.2019-02-01T07:24:44Z) https://github.com/owlcs/owlapi
